examples/AutoRewrite/DemoQuantPullRtac.v
@@ -65,7 +65,7 @@ Fixpoint count_quant (e : expr typ func) : nat :=
   end.
 
 Definition benchmark (n m : nat) : bool :=
-  match quant_pull (goal2 m n 0) (Rinj fImpl) nil nil nil 0 0 (TopSubst _ nil nil)
+  match quant_pull (goal2 m n 0) (Rinj fImpl) nil (TopSubst _ nil nil)
   with
   | Some _ => true
   | _ => false
